src/Ex/Mesi/MesiTopo.v
@@ -1,0 +1,336 @@
+Require Import Bool Vector List String Peano_dec Omega.
+Require Import Common FMap HVector ListSupport Syntax Topology Semantics.
+Require Import RqRsLang.
+
+Require Import Ex.Spec Ex.SpecSv Ex.ImplTemplate Ex.Mesi.
+Require Import Ex.Mesi.Mesi.
+
+Set Implicit Arguments.
+
+Local Open Scope list.
+Local Open Scope hvec.
+Local Open Scope fmap.
+
+(** TODO: move to [RqRsLang.v] *)
+Lemma initORqs_GoodORqsInit: forall oinds, GoodORqsInit (initORqs oinds).
+Proof.
+  red; intros.
+  unfold initORqs.
+  remember (M.empty (M.t (RqInfo Msg))) as m.
+  assert (forall oidx, m@[oidx] >>=[True] (fun orq => orq = []))
+    by (intros; subst; mred).
+  clear Heqm.
+  generalize dependent m.
+  induction oinds; simpl; intros; [auto|].
+  apply IHoinds.
+  intros.
+  mred; auto.
+Qed.
+
+(** TODO: move to [ListSupport.v] *)
+Lemma collect_forall:
+  forall {A B} P (f: A -> list B) al,
+    (forall a, In a al -> Forall P (f a)) ->
+    Forall P (collect f al).
+Proof.
+  induction al; intros; [constructor|].
+  simpl; apply Forall_app.
+  - apply H; left; reflexivity.
+  - apply IHal; intros.
+    apply H; right; assumption.
+Qed.
+
+Lemma collect_In:
+  forall {A B} (f: A -> list B) al b,
+    In b (collect f al) ->
+    exists a, In a al /\ In b (f a).
+Proof.
+  induction al; intros; [dest_in|].
+  simpl in H; apply in_app_or in H; destruct H.
+  - eexists; split; [left; reflexivity|assumption].
+  - specialize (IHal _ H).
+    destruct IHal as [na [? ?]].
+    eexists; split; [right; eassumption|assumption].
+Qed.
+
+Lemma incMap_In:
+  forall {A B} (f: A -> IdxT -> B) al base ext b,
+    In b (incMap f al base ext) ->
+    exists a extb, In a al /\ b = f a (base~>extb).
+Proof.
+  induction al; simpl; intros; [exfalso; auto|].
+  destruct H; subst; eauto.
+  specialize (IHal _ _ _ H).
+  destruct IHal as [pa [extb ?]]; dest; subst; eauto.
+Qed.
+
+Lemma app_eq_compare:
+  forall {A} (l m n o: list A),
+    l ++ m = n ++ o ->
+    exists p, (l = n ++ p /\ o = p ++ m) \/
+              (n = l ++ p /\ m = p ++ o).
+Proof.
+  induction l; simpl; intros.
+  - subst; eexists; right; eauto.
+  - destruct n as [|b n].
+    + simpl in *; subst.
+      eexists; left; eauto.
+    + simpl in H; inv H.
+      specialize (IHl _ _ _ H2).
+      destruct IHl as [p ?]; destruct H; dest; subst; [|eauto].
+      eexists; left; split; reflexivity.
+Qed.
+
+(** TODO: move to [Index.v] *)
+Definition IdxPrefix (i1 i2: IdxT) :=
+  exists ri, i2 = ri ++ i1.
+Infix "~<" := IdxPrefix (at level 8).
+
+Definition IdxDisj (i1 i2: IdxT) :=
+  ~ IdxPrefix i1 i2 /\ ~ IdxPrefix i2 i1.
+Infix "~*~" := IdxDisj (at level 8).
+
+Definition IndsDisj (is1 is2: list IdxT) :=
+  forall i1 i2, In i1 is1 -> In i2 is2 -> i1 ~*~ i2.
+
+Lemma extendIdx_not_IdxPrefix:
+  forall i e, ~ i~>e ~< i.
+Proof.
+  unfold extendIdx, IdxPrefix; intros.
+  intro Hx; dest.
+  replace (x ++ e :: i) with ((x ++ [e]) ++ i) in H
+    by (rewrite <-app_assoc; reflexivity).
+  remember (x ++ [e]) as l.
+  assert (l <> nil) by (intro Hx; subst; destruct x; discriminate).
+  clear Heql x e.
+  generalize dependent l.
+  induction i; simpl; intros.
+  - rewrite app_nil_r in H; auto.
+  - destruct l; [auto|].
+    inv H.
+    eapply IHi with (l:= l ++ [n]).
+    + rewrite <-app_assoc; assumption.
+    + destruct l; discriminate.
+Qed.
+
+Lemma IdxPrefix_refl: forall i, i ~< i.
+Proof.
+  unfold IdxPrefix; intros.
+  exists nil; reflexivity.
+Qed.
+
+Lemma IdxPrefix_trans:
+  forall i1 i2, i1 ~< i2 -> forall i3, i2 ~< i3 -> i1 ~< i3.
+Proof.
+  unfold IdxPrefix; intros; dest; subst.
+  eexists; rewrite app_assoc; reflexivity.
+Qed.
+
+Lemma IdxDisj_not_eq:
+  forall i1 i2, i1 ~*~ i2 -> i1 <> i2.
+Proof.
+  intros; intro Hx; subst.
+  red in H; dest.
+  elim H; apply IdxPrefix_refl.
+Qed.
+  
+Lemma IdxPrefix_common:
+  forall i1 i2 i, i1 ~< i -> i2 ~< i -> i1 ~< i2 \/ i2 ~< i1.
+Proof.
+  unfold IdxPrefix; intros; dest; subst.
+  apply app_eq_compare in H0.
+  destruct H0 as [p ?]; destruct H; dest; subst; eauto.
+Qed.
+
+Lemma IdxPrefix_disj_1:
+  forall i1 i2, i1 ~*~ i2 -> forall ei1, i1 ~< ei1 -> ei1 ~*~ i2.
+Proof.
+  unfold IdxDisj; intros; dest.
+  split.
+  - intro Hx; elim H.
+    eapply IdxPrefix_trans; eauto.
+  - intro Hx.
+    pose proof (IdxPrefix_common H0 Hx).
+    destruct H2; auto.
+Qed.
+
+Lemma IdxPrefix_disj_2:
+  forall i1 i2, i1 ~*~ i2 -> forall ei2, i2 ~< ei2 -> i1 ~*~ ei2.
+Proof.
+  unfold IdxDisj; intros; dest.
+  split.
+  - intro Hx.
+    pose proof (IdxPrefix_common H0 Hx).
+    destruct H2; auto.
+  - intro Hx; elim H1.
+    eapply IdxPrefix_trans; eauto.
+Qed.
+
+Lemma IdxDisj_base_IndsDisj:
+  forall bidx1 bidx2,
+    bidx1 ~*~ bidx2 ->
+    forall inds1 inds2,
+      Forall (fun idx => bidx1 ~< idx) inds1 ->
+      Forall (fun idx => bidx2 ~< idx) inds2 ->
+      IndsDisj inds1 inds2.
+Proof.
+  intros.
+  rewrite Forall_forall in H0, H1.
+  red; intros.
+  specialize (H0 _ H2); specialize (H1 _ H3).
+  eapply IdxPrefix_disj_1; [|eassumption].
+  eapply IdxPrefix_disj_2; [|eassumption].
+  assumption.
+Qed.
+
+Lemma IndsDisj_DisjList:
+  forall inds1 inds2, IndsDisj inds1 inds2 -> DisjList inds1 inds2.
+Proof.
+  unfold IndsDisj, DisjList; intros.
+  destruct (in_dec idx_dec e inds1); [|auto].
+  destruct (in_dec idx_dec e inds2); [|auto].
+  specialize (H _ _ i i0).
+  exfalso; eapply IdxDisj_not_eq; eauto.
+Qed.
+
+(** TODO: move to [ImplTemplate.v] *)
+Lemma singletonDNode_inds_prefix_base:
+  forall bidx,
+    Forall (fun idx => bidx ~< idx)
+           (indsOf (fst (singletonDNode bidx))).
+Proof.
+  intros; simpl.
+  repeat constructor.
+  - apply IdxPrefix_refl.
+  - exists [0]; reflexivity.
+Qed.
+
+Lemma tree2Topo_inds_prefix_base:
+  forall tr bidx,
+    Forall (fun idx => bidx ~< idx)
+           (indsOf (fst (tree2Topo tr bidx))).
+Proof.
+  induction tr using tree_ind_l.
+  intros; simpl.
+  destruct l.
+  - apply singletonDNode_inds_prefix_base.
+  - inv H.
+    simpl; constructor.
+    + apply IdxPrefix_refl.
+    + apply Forall_app.
+      * specialize (H2 bidx~>0).
+        eapply Forall_impl; [|eassumption].
+        simpl; intros.
+        eapply IdxPrefix_trans; [|eassumption].
+        exists [0]; reflexivity.
+      * apply collect_forall.
+        intros dstr ?.
+        apply in_map_iff in H.
+        destruct H as [[dtr sifc] [? ?]]; simpl in *; subst.
+        apply incMap_In in H0.
+        destruct H0 as [str [extb ?]]; dest.
+        rewrite Forall_forall in H3; specialize (H3 _ H bidx~>extb).
+        rewrite <-H0 in H3; simpl in H3.
+        eapply Forall_impl; [|eassumption].
+        simpl; intros.
+        eapply IdxPrefix_trans; [|eassumption].
+        exists [extb]; reflexivity.
+Qed.
+
+Lemma tree2Topo_disj_inds:
+  forall tr1 bidx1 tr2 bidx2,
+    bidx1 ~*~ bidx2 ->
+    DisjList (indsOf (fst (tree2Topo tr1 bidx1)))
+             (indsOf (fst (tree2Topo tr2 bidx2))).
+Proof.
+  intros.
+  apply IndsDisj_DisjList.
+  eapply IdxDisj_base_IndsDisj; [eassumption|..];
+    apply tree2Topo_inds_prefix_base.
+Qed.
+
+Lemma l1ExtOf_not_eq:
+  forall bidx, l1ExtOf bidx <> bidx.
+Proof.
+  intros; induction bidx; [discriminate|].
+  intro Hx; inv Hx; auto.
+Qed.
+
+Lemma singletonDNode_WfDTree:
+  forall bidx, WfDTree (fst (singletonDNode bidx)).
+Proof.
+  intros; split.
+  - red; simpl.
+    repeat constructor; intro Hx; dest_in.
+    unfold l1ExtOf, extendIdx in H.
+    eapply l1ExtOf_not_eq; eauto.
+  - red; simpl.
+    match goal with
+    | |- NoDup (?i1 :: ?i2 :: ?i3 :: ?inds) =>
+      change (i1 :: i2 :: i3 :: inds) with ([i1; i2; i3] ++ inds)
+    end.
+    apply NoDup_DisjList.
+    + solve_NoDup.
+    + solve_NoDup.
+    + match goal with
+      | |- DisjList ?ll _ =>
+        let e := fresh "e" in
+        red; intro e; destruct (in_dec idx_dec e ll); [right|auto]; dest_in;
+          intro Hx; dest_in; try discriminate
+      end.
+      * inv H; eapply l1ExtOf_not_eq; eauto.
+      * inv H0; eapply l1ExtOf_not_eq; eauto.
+      * inv H; eapply l1ExtOf_not_eq; eauto.
+Qed.
+
+Lemma tree2Topo_WfDTree:
+  forall tr bidx, WfDTree (fst (tree2Topo tr bidx)).
+Proof.
+  induction tr using tree_ind_l.
+  intros; simpl.
+  destruct l.
+  - apply singletonDNode_WfDTree.
+  - remember (t :: l) as strs; clear Heqstrs t l.
+    simpl; split.
+    + red; simpl.
+      constructor.
+      * intro Hx; apply collect_In in Hx.
+        destruct Hx as [a [? ?]].
+        apply in_map_iff in H0; destruct H0 as [[dtr cifc] [? ?]].
+        simpl in *; subst.
+        apply incMap_In in H2.
+        destruct H2 as [str [extb ?]]; dest.
+        pose proof (tree2Topo_inds_prefix_base str bidx~>extb).
+        rewrite <-H2 in H3; simpl in H3.
+        rewrite Forall_forall in H3; specialize (H3 _ H1).
+        eapply extendIdx_not_IdxPrefix; eassumption.
+      * admit.
+    + red; simpl.
+      match goal with
+      | |- NoDup (?i1 :: ?i2 :: ?i3 :: ?inds) =>
+        change (i1 :: i2 :: i3 :: inds) with ([i1; i2; i3] ++ inds)
+      end.
+      apply NoDup_DisjList.
+      * solve_NoDup.
+      * admit.
+      * admit.
+Admitted.
+
+Section System.
+  Variable tr: tree.
+
+  Local Definition topo := fst (tree2Topo tr 0).
+  Local Definition cifc := snd (tree2Topo tr 0).
+
+  Lemma mesi_impl_ORqsInit: GoodORqsInit (initsOf (impl tr)).
+  Proof.
+    apply initORqs_GoodORqsInit.
+  Qed.
+
+  Lemma mesi_topo_wf: WfDTree topo.
+  Proof.
+    apply tree2Topo_WfDTree.
+  Qed.
+
+End System.
+
